change AsVal to be easier to use (like IntoVal)

theories/program_logic/language.v
@@ -162,12 +162,12 @@ Section language.
   Class IntoVal (e : expr Λ) (v : val Λ) :=
     into_val : of_val v = e.
 
-  Class AsVal (e : expr Λ) := as_val : is_Some (to_val e).
+  Class AsVal (e : expr Λ) := as_val : ∃ v, of_val v = e.
   (* There is no instance [IntoVal → AsVal] as often one can solve [AsVal] more
   efficiently since no witness has to be computed. *)
   Global Instance as_vals_of_val vs : TCForall AsVal (of_val <$> vs).
   Proof.
     apply TCForall_Forall, Forall_fmap, Forall_true=> v.
-    rewrite /AsVal /= to_of_val; eauto.
+    rewrite /AsVal /=; eauto.
   Qed.
 End language.
